fixed some issues

projectVampire/dafny/blood.dfy
@@ -1,3 +1,4 @@
+
 // state:
 // unsafe = -1
 // unverified = 0
@@ -139,3 +140,142 @@ class Blood{
     ensures Valid()
     {state:=unsafe;}
 }
+
+//#include blood.dfy
+
+class transportationManager {
+	
+	var locale: int; // give each location an int value?
+	var destinations: array<int>; //:= new int[10]; // routes to destinations
+	var toSend: array<Blood>;// := new Blood[10]; // may need to have another array that matches the blood destinations to each index or create a class that can hold blood and its dest
+    	var toDest: array<int>;// := new int[10]; // routes (match with toSend array)
+
+    	
+
+	// Blood always has a destination, ie every blood in array is matched by a route
+	predicate method Valid()
+	//requires toDest != null;
+	//requires toSend != null
+	reads this;
+	//reads toDest[0],toDest[1], toDest[2],toDest[3],toDest[4],toDest[5],toDest[6],toDest[7],toDest[8],toDest[9];
+	requires toDest != null;
+	requires toSend != null;
+	{
+        	//forall x,y:: 0 <= x < toDest.Length && 0 <= y < toSend.Length && x == y ==> toDest[x]!=-1 && toSend[y] != null
+    		toDest !=null && toSend != null
+	}
+
+
+	method Init(src: int)
+	modifies this;
+	modifies toDest;
+	modifies toSend;
+	modifies `locale;
+	requires src >= 0
+	ensures toDest != null;
+	ensures toSend != null;
+	ensures Valid()
+	{
+		locale := src;
+		toDest := new int[10];
+		toSend := new Blood[10];
+		//var i := 0;
+		//assert toSend != null;
+		//while (i < toSend.Length) 
+		//invariant 0 <= i < toSend.Length
+		//{	
+		//	toSend[i] := null;
+		//	i := i + 1;
+		//}
+		//i := 0;
+		//while (i < toDest.Length)
+		//invariant 0 <= i < toDest.Length
+		//{
+		//	toDest[i] := -1;
+		//	i := i + 1;
+		//}
+	}
+
+		
+	method receive(bld:Blood, dst:int)
+	modifies this.toDest
+	modifies this.toSend 
+	requires toSend != null
+	requires toDest != null
+	requires forall x :: 0 <= x < toSend.Length ==> bld != toSend[x] // blood is not already in toSend
+	requires bld != null;
+	requires toSend.Length == toDest.Length
+	requires dst >= 0;
+	requires Valid(); ensures Valid();
+	//ensures forall x, y:: 0 <= x < toSend.Length && 0 <= y < toDest.Length && x == y ==> toSend[x] == bld && toDest[y] == dst -> need to fix
+	{
+       		var cDest := -1;
+		if (dst == -1) {
+			cDest := 3; // need to grab the dest that system spits out
+		} else {
+			cDest := -1;
+		}
+		//var index := 0;
+		//var i := 0;
+		//while (index < toSend.Length) 
+		//invariant 0 <= i <= toSend.Length
+		//{
+		//	if (toSend[i] == null) {
+		//		index := i;
+		//		i := toSend.Length -1;		
+		//	}
+		//	i :=  i + 1;
+		//}
+		//toSend[i] := bld;
+		//toDest[i] := cDest;
+
+		var i := 0;
+		var j := 0;
+		while (i < toSend.Length && j < toDest.Length)
+		invariant 0 <= i <= toSend.Length
+		invariant 0 <= j <= toDest.Length
+		//invariant forall x,y :: 0 <= x < toSend.Length && 0 <= y < toDest.Length && toDest[y] == cDest && toSend[x] == bld ==> (x==y) -> need to fix
+		//invariant forall x :: 0 <= x < (j-1) ==> toDest[x] != 0
+		//invariant forall x, y :: 0 <= x < i && 0 <= y < j && x == y ==> toSend[x] == bl
+		invariant i == j
+		{
+			if (toSend[i] == null && toDest[j] == 0) {
+				toSend[i] := bld;
+				toDest[j] := cDest;
+				//i := toSend.Length -1;
+				//j := toDest.Length -1;
+			}
+			i := i + 1;
+			j := j + 1;
+		}
+    	}
+
+
+	method dispatchBlood()
+	modifies toSend;
+	modifies toDest;
+	requires toSend != null;
+	requires toDest != null;
+	requires exists x :: 0 <= x < toSend.Length && toSend[x] != null // blood is to be sent
+	requires Valid();ensures Valid();
+    	ensures forall x, y:: 0 <= x < toSend.Length && 0 <= y < toDest.Length  && x == y ==> (toSend[x] == null && toDest[y] == 0) // toSend and toRoute are empty
+	{
+		var i := 0;
+		var j := 0;
+		while (i < toSend.Length && j < toDest.Length)
+		invariant 0 <= i <= toSend.Length
+		invariant 0 <= j <= toDest.Length
+		invariant forall x :: 0 <= x < i ==> toSend[x] == null
+		invariant forall x :: 0 <= x < j ==> toDest[x] == 0
+		invariant i == j
+		{
+			toDest[j] := 0;
+			toSend[i] := null;
+			i := i + 1;
+			j := j + 1;
+		}
+		
+    	}
+    
+}
+
